\documentclass{article}
\usepackage{ifthen}
\usepackage{epsfig}
\usepackage[utf8]{inputenc}
\usepackage{newunicodechar}
  \newunicodechar{⁻}{${}^{-}$}% Superscript minus
  \newunicodechar{²}{${}^{2}$}% Superscript two
  \newunicodechar{³}{${}^{3}$}% Superscript three

\pagestyle{empty}
\begin{document}
\[ x_{i+1}\leftarrow(ax_{i} + c) \bmod m \]
\pagebreak

$1$
\pagebreak

\[ x_{i}\leftarrow(x_{i - s} - x_{i - r} - carry_{i-1}) \bmod m \]
\pagebreak

$r$
\pagebreak

$(m^r - m^s - 1)$
\pagebreak

$x_0$
\pagebreak

$ m_{lcg} = 2147483563, a_{lcg} = 40014, c_{lcg} = 0, and lcg(0) = value $
\pagebreak

$ x_{-r} \dots x_{-1} $
\pagebreak

$ lcg(1) \bmod m \dots lcg(r) \bmod m $
\pagebreak

$ x_{-1} = 0 $
\pagebreak

$[min, max]$
\pagebreak

\[ p(x|\mu,\sigma) = \frac{1}{\sigma \sqrt{2 \pi}} e^{- \frac{{x - \mu}^ {2}}{2 \sigma ^ {2}} } \]
\pagebreak

$mean$
\pagebreak

\[ p(x|m,s) = \frac{1}{sx\sqrt{2\pi}} \exp{-\frac{(\ln{x} - m)^2}{2s^2}} \]
\pagebreak

\[ p(x|\alpha,\beta) = \frac{1}{\beta\Gamma(\alpha)} (x/\beta)^{\alpha - 1} e^{-x/\beta} \]
\pagebreak

$\alpha$
\pagebreak

$\beta$
\pagebreak

$p(x|n) = \frac{x^{(n/2) - 1}e^{-x/2}}{\Gamma(n/2) 2^{n/2}}$
\pagebreak

$p(x|a,b) = (\pi b (1 + (\frac{x-a}{b})^2))^{-1}$
\pagebreak

\[ p(x|m,n) = \frac{\Gamma((m+n)/2)}{\Gamma(m/2)\Gamma(n/2)} (\frac{m}{n})^{m/2} x^{(m/2)-1} (1 + \frac{mx}{n})^{-(m+n)/2} \]
\pagebreak

\[ p(x|n) = \frac{1}{\sqrt(n\pi)} \frac{\Gamma((n+1)/2)}{\Gamma(n/2)} (1 + \frac{x^2}{n}) ^{-(n+1)/2} \]
\pagebreak

$p$
\pagebreak

$(1 - p)$
\pagebreak

$[0, 1]$
\pagebreak

$p(i|t,p) = \binom{n}{i} p^i (1 - p)^{t - i}$
\pagebreak

$t$
\pagebreak

$p(i|p) = p(1 - p)^{i}$
\pagebreak

$p(i) = \binom{n}{i} p^i (1 - p)^{t - i}$
\pagebreak

$k$
\pagebreak

$p(i|\mu) = \frac{\mu^i}{i!} e^{-\mu}$
\pagebreak

$\mu$
\pagebreak

$p(x|\lambda) = \lambda e^{-\lambda x}$
\pagebreak

$\frac{1}{\lambda}$
\pagebreak

$\frac{\ln 2}{\lambda}$
\pagebreak

$zero$
\pagebreak

$[0, \infty]$
\pagebreak

$\lambda$
\pagebreak

\[ p(x|\alpha,\beta) = \frac{\alpha}{\beta} (\frac{x}{\beta})^{\alpha-1} \exp{(-(\frac{x}{\beta})^\alpha)} \]
\pagebreak

$a$
\pagebreak

$b$
\pagebreak

\[ p(x|a,b) = \frac{1}{b} \exp( \frac{a-x}{b} - \exp(\frac{a-x}{b})) \]
\pagebreak

$x_{i+1}\leftarrow(ax_{i} + c) \bmod m $
\pagebreak

$ 1 $
\pagebreak

$x_{i}\leftarrow(x_{i - s} - x_{i - r} - carry_{i-1}) \bmod m $
\pagebreak

$ r $
\pagebreak

$ m^r - m^s -1 $
\pagebreak

$ x_0 $
\pagebreak

$(min, max)$
\pagebreak

$[0, n)$
\pagebreak

$ p $
\pagebreak

$ (1 - p) $
\pagebreak

$ [0, 1] $
\pagebreak

$ p(i) = (1 - p)p^{i-1} $
\pagebreak

$ p(i) = \frac{mean^i}{i!} e^{-mean} $
\pagebreak

$ mean $
\pagebreak

$ p(i) = \binom{n}{i} p^i (1 - p)^{t - i} $
\pagebreak

$ t $
\pagebreak

$ p(x) = \lambda e^{-\lambda x} $
\pagebreak

$ \frac{1}{\lambda} $
\pagebreak

$ \frac{\ln 2}{\lambda} $
\pagebreak

$ zero $
\pagebreak

$ \lambda $
\pagebreak

$ p(x) = \frac{1}{\sigma \sqrt{2 \pi}} e^{- \frac{{x - mean}^ {2}}{2 \sigma ^ {2}} } $
\pagebreak

$ \sigma $
\pagebreak

$ p(x) = \frac{1}{\Gamma(\alpha)} x^{\alpha - 1} e^{-x} $
\pagebreak

$ \alpha $
\pagebreak

$ \pi $
\pagebreak

$ \pi / 2 $
\pagebreak

$ \pi / 3 $
\pagebreak

$ \pi / 4 $
\pagebreak

$ 1 / \pi $
\pagebreak

$ 2 / \sqrt(\pi) $
\pagebreak

$ \sqrt(2) $
\pagebreak

$ \sqrt(3) $
\pagebreak

$ \sqrt(\pi/2) $
\pagebreak

$ 1 / sqrt(2) $
\pagebreak

$ \log(\pi) $
\pagebreak

$ \gamma_E $
\pagebreak

$ e $
\pagebreak

\end{document}
